refactor: closure automation

stdlib/iterator/src/adapters/map.rs
@@ -35,12 +35,12 @@ impl<I, F> Map<I, F>
 }
 
 /// Spec: We have the pure parts of the inner Next and the pre- and postconditions.
-#[rr::instantiate("Params" := "({MI::Params} * ({MF::Params} → Prop))%type")]
+#[rr::instantiate("Params" := "({MI::Params} * (RT_xt (tuple1_rt {rt_of MI::Item}) → {MF::Params} → Prop))%type")]
 #[rr::instantiate("Next" := "(λ π '(p_inner, ParamPred) s1 e s2, 
         if_iNone e ({MI::Next} π p_inner s1.(map_it) None s2.(map_it)) ∗
         if_iSome e (λ e, ∃ e_inner,
             ({MI::Next} π p_inner s1.(map_it) (Some e_inner) s2.(map_it)) ∗
-            ∃ p_clos, ⌜ParamPred p_clos⌝ ∗ boringly ({MF::Pre} π p_clos s1.(map_clos) *[e_inner]) ∗
+            ∃ p_clos, ⌜ParamPred *[e_inner] p_clos⌝ ∗ boringly ({MF::Pre} π p_clos s1.(map_clos) *[e_inner]) ∗
             ({MF::PostMut} π p_clos s1.(map_clos) *[e_inner] s2.(map_clos) e)
             ))%I")]
 #[rr::instantiate("Inv" := "MapInv traits_iterator_Iterator_MI_spec_attrs {MF::Pre} {MF::PostMut}")]
