stdlib/closures/theories/simplification.v
@@ -4,6 +4,8 @@ From refinedrust Require Import typing.
 (** Inspired by Quiver's simplification machinery:
    https://gitlab.mpi-sws.org/simonspies/quiver/-/blob/4c63760910c39373032b5dab1d78a181bdc8ad53/theories/argon/simplification/elim_existentials.v *)
 
+Local Set Typeclasses Unique Instances.
+
 (** A typeclass to check whether a relation is the identity relation *)
 Class RelationIsIdentity {A} (R : A → A → Prop) := {
   relation_is_identity_proof : ∀ a b, R a b → a = b;
@@ -21,114 +23,133 @@ Global Hint Extern 100 (RelationIsFunctional _ _) =>
     repeat (liForall || liImpl); done : typeclass_instances.
 Global Hint Mode RelationIsIdentity + - : typeclass_instances.
 
+Definition cnf Cs := fold_right and True Cs.
+
+Lemma cnf_app Cs1 Cs2 :
+  cnf (Cs1 ++ Cs2) ↔ cnf Cs1 ∧ cnf Cs2.
+Proof.
+  rewrite /cnf. induction Cs1 as [ | C1 Cs1 IH]; simpl; naive_solver.
+Qed.
+
 Definition simplify_prop (P R : Prop) := P ↔ R.
 Section bubble_existentials.
 
   Implicit Types (P Q R : Prop).
   Implicit Types (A : Type).
 
-  Definition bubble_existentials P R Q := (P ∧ Q) ↔ R.
+  Definition bubble_existentials (worklist : list Prop) Cs R (prog : bool) :=
+    (cnf worklist ∧ cnf Cs) ↔ R.
+  Global Hint Mode bubble_existentials + + - - : typeclass_instances.
 
-  Lemma bubble_existentials_and_ex_l A Φ Ψ Q Acc :
-    (∀ x : A, bubble_existentials (Φ x ∧ Q) (Ψ x) Acc) →
-    bubble_existentials ((∃ x : A, Φ x) ∧ Q) (∃ x : A, Ψ x) Acc.
+  (* this doesn't work so well in practice.
+    Ideally, i should also normalize to cnf now.
+
+    Let's do a DFS (leftmost).
+    Put RHS conjuncts on a worklist.
+
+  *)
+  Lemma bubble_existentials_and P Q worklist Cs R prog :
+    bubble_existentials (P :: Q :: worklist) Cs R prog →
+    bubble_existentials ((P ∧ Q) :: worklist) Cs R prog.
+  Proof.
+    rewrite /bubble_existentials/simplify_prop/=. naive_solver.
+  Qed.
+
+  (* we made progress if there are some conjuncts on the output list already *)
+  Lemma bubble_existentials_exist_no_prog A Φ Ψ worklist prog  :
+    (∀ x : A, bubble_existentials (Φ x :: worklist) [] (Ψ x) prog) →
+    bubble_existentials ((∃ x : A, Φ x) :: worklist) [] (∃ x : A, Ψ x) (prog).
+  Proof.
+    rewrite /bubble_existentials/simplify_prop. naive_solver.
+  Qed.
+  Lemma bubble_existentials_exist A Φ Ψ Cs worklist prog  :
+    TCDone (Cs ≠ []) →
+    (∀ x : A, bubble_existentials (Φ x :: worklist) Cs (Ψ x) prog) →
+    bubble_existentials ((∃ x : A, Φ x) :: worklist) Cs (∃ x : A, Ψ x) true.
   Proof.
     rewrite /bubble_existentials/simplify_prop. naive_solver.
   Qed.
 
-  Lemma bubble_existentials_shelve_l P Q R Acc :
-    bubble_existentials Q R (P ∧ Acc) →
-    bubble_existentials (P ∧ Q) R Acc.
+  Lemma bubble_existentials_nil Cs :
+    bubble_existentials [] Cs (cnf Cs) false.
   Proof.
-    rewrite /bubble_existentials. naive_solver.
+    rewrite /bubble_existentials/simplify_prop/=. naive_solver.
   Qed.
 
-  Lemma bubble_existentials_ex A Φ Ψ Acc :
-    (∀ x : A, bubble_existentials (Φ x) (Ψ x) Acc) →
-    bubble_existentials (∃ x : A, Φ x) (∃ x : A, Ψ x) Acc.
+  Lemma bubble_existentials_atom worklist P Cs R prog :
+    bubble_existentials worklist (P :: Cs) R prog →
+    bubble_existentials (P :: worklist) Cs R prog.
   Proof.
-    rewrite /bubble_existentials/simplify_prop.
-    naive_solver.
-  Qed.
-
-  Lemma bubble_existentials_atom P Acc :
-    bubble_existentials P (P ∧ Acc) Acc.
-  Proof.
-    rewrite /bubble_existentials/simplify_prop. naive_solver.
+    rewrite /bubble_existentials/simplify_prop/=. naive_solver.
   Qed.
 End bubble_existentials.
 
 Global Typeclasses Opaque bubble_existentials.
 Existing Class bubble_existentials.
 
-Existing Instances bubble_existentials_and_ex_l | 1.
-Existing Instances bubble_existentials_shelve_l | 10.
-Existing Instance bubble_existentials_ex.
-Existing Instance bubble_existentials_atom | 1000.
+Global Existing Instances bubble_existentials_and | 1.
+(* use [eapply] for better unification *)
+Global Hint Extern 1 (bubble_existentials _ _ _ _) => eapply bubble_existentials_exist_no_prog : typeclass_instances.
+Global Hint Extern 10 (bubble_existentials _ (_ :: _) _ _) => eapply bubble_existentials_exist : typeclass_instances.
+Global Existing Instance bubble_existentials_nil | 1.
+Global Existing Instance bubble_existentials_atom | 100.
 
 Section normalize_conjuncts.
   Implicit Types (P Q R : Prop).
   Implicit Types (A : Type).
   Implicit Type (Cs : list Prop).
 
-  Definition cnf Cs := fold_right and True Cs.
 
-  Lemma cnf_app Cs1 Cs2 :
-    cnf (Cs1 ++ Cs2) ↔ cnf Cs1 ∧ cnf Cs2.
-  Proof.
-    rewrite /cnf. induction Cs1 as [ | C1 Cs1 IH]; simpl; naive_solver.
-  Qed.
+  Definition normalize_conjuncts P R (prog : bool) := simplify_prop P R.
+  Definition normalize_as_conjuncts Cs Cs' (prog : bool) := simplify_prop (cnf Cs) (cnf Cs').
 
-  Definition normalize_conjuncts P R := simplify_prop P R.
-  Definition normalize_as_conjuncts P Cs := simplify_prop P (cnf Cs).
-
-  Lemma normalize_conjuncts_exists A Φ Ψ :
-    (∀ x : A, normalize_conjuncts (Φ x) (Ψ x)) →
-    normalize_conjuncts (∃ x : A, Φ x) (∃ x : A, Ψ x).
+  Lemma normalize_conjuncts_exists A Φ Ψ prog :
+    (∀ x : A, normalize_conjuncts (Φ x) (Ψ x) prog) →
+    normalize_conjuncts (∃ x : A, Φ x) (∃ x : A, Ψ x) prog.
   Proof.
     rewrite /normalize_conjuncts /simplify_prop.
     naive_solver.
   Qed.
 
-  Lemma normalize_conjuncts_exists_unused A `{!Inhabited A} P R :
-    normalize_conjuncts P R →
-    normalize_conjuncts (∃ x : A, P) (R).
+  Lemma normalize_conjuncts_exists_unused A `{!Inhabited A} P R prog :
+    normalize_conjuncts P R prog →
+    normalize_conjuncts (∃ x : A, P) (R) true.
   Proof.
     rewrite /normalize_conjuncts /simplify_prop.
     intros <-.
     split; first naive_solver.
     intros. exists inhabitant. done.
   Qed.
-  Lemma normalize_conjuncts_exists_unit Φ R :
-    normalize_conjuncts (Φ tt) R →
-    normalize_conjuncts (∃ x : unit, Φ x) (R).
+  Lemma normalize_conjuncts_exists_unit Φ R prog :
+    normalize_conjuncts (Φ tt) R prog →
+    normalize_conjuncts (∃ x : unit, Φ x) (R) true.
   Proof.
     rewrite /normalize_conjuncts /simplify_prop.
     intros <-.
     split; last naive_solver.
     intros [[] ?]. done.
   Qed.
-  Lemma normalize_conjuncts_exists_nil_unit Φ R :
-    normalize_conjuncts (Φ *[]) R →
-    normalize_conjuncts (∃ x : nil_unit, Φ x) (R).
+  Lemma normalize_conjuncts_exists_nil_unit Φ R prog :
+    normalize_conjuncts (Φ *[]) R prog →
+    normalize_conjuncts (∃ x : nil_unit, Φ x) (R) true.
   Proof.
     rewrite /normalize_conjuncts /simplify_prop.
     intros <-.
     split; last naive_solver.
     intros [[] ?]. done.
   Qed.
-  Lemma normalize_conjuncts_exists_plist_cons {A} (F : A → Type) (X : A) Xs Φ R :
-    normalize_conjuncts (∃ x1 : F X, ∃ x2 : plist F Xs, Φ ( x1 -:: x2)) R →
-    normalize_conjuncts (∃ x : plist F (X :: Xs), Φ x) (R).
+  Lemma normalize_conjuncts_exists_plist_cons {A} (F : A → Type) (X : A) Xs Φ R prog :
+    normalize_conjuncts (∃ x1 : F X, ∃ x2 : plist F Xs, Φ ( x1 -:: x2)) R prog →
+    normalize_conjuncts (∃ x : plist F (X :: Xs), Φ x) (R) true.
   Proof.
     rewrite /normalize_conjuncts /simplify_prop.
     intros <-.
     split; last naive_solver.
     intros [[] ?]. eauto.
   Qed.
-  Lemma normalize_conjuncts_exists_plist_nil {A} (F : A → Type) Φ R :
-    normalize_conjuncts (Φ -[]) R →
-    normalize_conjuncts (∃ x : plist F [], Φ x) (R).
+  Lemma normalize_conjuncts_exists_plist_nil {A} (F : A → Type) Φ R prog :
+    normalize_conjuncts (Φ -[]) R prog →
+    normalize_conjuncts (∃ x : plist F [], Φ x) (R) true.
   Proof.
     rewrite /normalize_conjuncts /simplify_prop.
     intros <-.
@@ -136,59 +157,60 @@ Section normalize_conjuncts.
     intros [[] ?]. done.
   Qed.
 
-  Lemma normalize_conjuncts_as_conjuncts P Cs :
-    normalize_as_conjuncts P Cs →
-    normalize_conjuncts P (cnf Cs).
+  Lemma normalize_conjuncts_as_conjuncts Cs Cs' prog :
+    normalize_as_conjuncts Cs Cs' prog →
+    normalize_conjuncts (cnf Cs) (cnf Cs') prog.
   Proof.
     rewrite /normalize_conjuncts /normalize_as_conjuncts /simplify_prop.
     naive_solver.
   Qed.
 
-  Lemma normalize_as_conjuncts_and P Q Cs1 Cs2 :
-    normalize_as_conjuncts P Cs1 →
-    normalize_as_conjuncts Q Cs2 →
-    normalize_as_conjuncts (P ∧ Q) (Cs1 ++ Cs2).
+  Lemma normalize_as_conjuncts_nil :
+    normalize_as_conjuncts [] [] false.
   Proof.
     rewrite /normalize_as_conjuncts/simplify_prop.
-    rewrite cnf_app. naive_solver.
+    done.
   Qed.
 
-  Lemma normalize_as_conjuncts_trivial P :
+  Lemma normalize_as_conjuncts_trivial P Cs Cs' prog :
     TCFastDone P →
-    normalize_as_conjuncts P [].
+    normalize_as_conjuncts Cs Cs' prog →
+    normalize_as_conjuncts (P :: Cs) Cs' true.
   Proof.
     rewrite /normalize_as_conjuncts/simplify_prop.
     unfold TCFastDone.
-    simpl. done.
+    simpl. naive_solver.
   Qed.
 
-  Lemma normalize_as_conjuncts_unit_eq x :
-    normalize_as_conjuncts (x = tt) [].
+  Lemma normalize_as_conjuncts_unit_eq x Cs Cs' prog :
+    normalize_as_conjuncts Cs Cs' prog →
+    normalize_as_conjuncts ((x = tt) :: Cs) Cs' true.
   Proof.
     rewrite /normalize_as_conjuncts/simplify_prop.
     destruct x.
     naive_solver.
   Qed.
 
-  Lemma normalize_as_conjuncts_pair_eq {A B} (a1 a2 : A) (b1 b2 : B) Cs :
-    normalize_as_conjuncts (a1 = a2 ∧ b1 = b2) Cs →
-    normalize_as_conjuncts ((a1, b1) = (a2, b2)) Cs.
+  Lemma normalize_as_conjuncts_pair_eq {A B} (a1 a2 : A) (b1 b2 : B) Cs Cs' prog :
+    normalize_as_conjuncts ((a1 = a2) :: (b1 = b2) :: Cs) Cs' prog →
+    normalize_as_conjuncts (((a1, b1) = (a2, b2)) :: Cs) Cs' true.
   Proof.
     rewrite /normalize_as_conjuncts/simplify_prop.
     naive_solver.
   Qed.
 
   #[universes(polymorphic)]
-  Lemma normalize_as_conjuncts_pcons_eq {A C} (a1 a2 : A) (b1 b2 : C) Cs :
-    normalize_as_conjuncts (a1 = a2 ∧ b1 = b2) Cs →
-    normalize_as_conjuncts (a1 *:: b1 = a2 *:: b2) Cs.
+  Lemma normalize_as_conjuncts_pcons_eq {A C} (a1 a2 : A) (b1 b2 : C) Cs Cs' prog :
+    normalize_as_conjuncts ((a1 = a2) :: (b1 = b2) :: Cs) Cs' prog →
+    normalize_as_conjuncts ((a1 *:: b1 = a2 *:: b2) :: Cs) Cs' true.
   Proof.
     rewrite /normalize_as_conjuncts/simplify_prop.
     naive_solver.
   Qed.
 
-  Lemma normalize_as_conjuncts_keep P :
-    normalize_as_conjuncts P [P].
+  Lemma normalize_as_conjuncts_keep P Cs Cs' prog :
+    normalize_as_conjuncts Cs Cs' prog →
+    normalize_as_conjuncts (P :: Cs) (P :: Cs') prog.
   Proof.
     rewrite /normalize_as_conjuncts/simplify_prop.
     simpl. naive_solver.
@@ -205,7 +227,7 @@ Existing Instances normalize_conjuncts_exists_plist_cons normalize_conjuncts_exi
 Existing Instance normalize_conjuncts_exists | 99.
 Existing Instance normalize_conjuncts_as_conjuncts | 100.
 
-Existing Instance normalize_as_conjuncts_and | 1.
+Existing Instance normalize_as_conjuncts_nil.
 Existing Instance normalize_as_conjuncts_trivial | 10.
 Existing Instance normalize_as_conjuncts_unit_eq | 11.
 Existing Instance normalize_as_conjuncts_pair_eq | 20.
@@ -214,7 +236,7 @@ Existing Instance normalize_as_conjuncts_keep | 100.
 
 Section resolve_existentials.
 
-  Definition elim_existentials (P R : Prop) :=
+  Definition elim_existentials (P R : Prop) (prog : bool) :=
     simplify_prop P R.
 
   Definition elim_this_existential (P R : Prop) :=
@@ -262,21 +284,21 @@ Section resolve_existentials.
 
   (** Pick an existential to eliminate *)
   Lemma elim_existentials_finish P:
-    elim_existentials P P.
+    elim_existentials P P false.
   Proof. rewrite /elim_existentials/simplify_prop. done. Qed.
 
-  Lemma elim_existentials_exists_elim X F R R':
+  Lemma elim_existentials_exists_elim X F R R' prog :
     elim_this_existential (∃ x: X, F x) R →
-    elim_existentials R R' →
-    elim_existentials (∃ x: X, F x) R'.
+    elim_existentials R R' prog →
+    elim_existentials (∃ x: X, F x) R' true.
   Proof.
     rewrite /elim_this_existential /elim_existentials /simplify_prop //.
     naive_solver.
   Qed.
 
-  Lemma elim_existentials_exists_skip X (F G: X → Prop):
-    (∀ x, elim_existentials (F x) (G x)) →
-    elim_existentials (∃ x: X, F x) (∃ x: X, G x).
+  Lemma elim_existentials_exists_skip X (F G: X → Prop) prog :
+    (∀ x, elim_existentials (F x) (G x) prog) →
+    elim_existentials (∃ x: X, F x) (∃ x: X, G x) prog.
   Proof. rewrite /elim_existentials/simplify_prop. naive_solver. Qed.
 
   (** Eliminate an existential *)
@@ -344,50 +366,52 @@ Global Existing Instance unfold_cnf_nil | 10.
 
 Arguments cnf : simpl never.
 
-Definition simplify_closure_prop P Q := simplify_prop P Q.
+Definition simplify_closure_prop P Q (prog : bool) := simplify_prop P Q.
 
-Lemma simplify_closure_prop_simpl P1 P2 P3 P4 P5 :
-  bubble_existentials P1 P2 True →
-  normalize_conjuncts P2 P3 →
-  elim_existentials P3 P4 →
+Lemma simplify_closure_prop_simpl P1 P2 P3 P4 P5 prog1 prog2 prog3 :
+  bubble_existentials [P1] [] P2 prog1 →
+  normalize_conjuncts P2 P3 prog2 →
+  elim_existentials P3 P4 prog3 →
   unfold_cnf P4 P5 →
-  simplify_closure_prop P1 P5.
+  simplify_closure_prop P1 P5 (prog1 || prog2 || prog3).
 Proof.
   rewrite /bubble_existentials /normalize_conjuncts /elim_existentials /unfold_cnf /simplify_closure_prop /simplify_prop /=.
+  simpl. rewrite /cnf/=.
   naive_solver.
 Qed.
 
-Lemma simplify_closure_prop_replace Φ Φ' Ψ :
+Lemma simplify_closure_prop_replace Φ Φ' Ψ prog :
   Φ = Φ' →
-  simplify_closure_prop Φ' Ψ →
-  simplify_closure_prop Φ Ψ.
+  simplify_closure_prop Φ' Ψ prog →
+  simplify_closure_prop Φ Ψ prog.
 Proof.
   intros ->. done.
 Qed.
 
 Existing Class simplify_closure_prop.
-Global Hint Extern 10 (simplify_closure_prop _ _) =>
-  notypeclasses refine (simplify_closure_prop_simpl _ _ _ _ _ _ _ _ _);
+Global Hint Extern 10 (simplify_closure_prop _ _ _) =>
+  notypeclasses refine (simplify_closure_prop_simpl _ _ _ _ _ _ _ _ _ _ _ _);
   [simpl; typeclasses eauto | simpl; typeclasses eauto | simpl; typeclasses eauto | simpl; typeclasses eauto] : typeclass_instances.
 
-Hint Extern 1 (simplify_closure_prop _ _) =>
+Hint Extern 1 (simplify_closure_prop _ _ _) =>
   match goal with
   | |- (simplify_closure_prop (let (a, b) := ?p in ?Φ) ?P) =>
-      notypeclasses refine (simplify_closure_prop_replace _ (let a := fst p in let b := snd p in Φ) _ _ _);
+      notypeclasses refine (simplify_closure_prop_replace _ (let a := fst p in let b := snd p in Φ) _ _ _ _);
       [destruct p; done |  ]
   end : typeclass_instances.
 
 Section test.
   Lemma test_1 (a b : Z) :
-    ∃ P1 P2 P3 P4,
-      bubble_existentials (∃ pclos : plist id [], True ∧ (∃ (a0 : Z) (_ : gname), pclos = *[] ∧ *[a] = *[a0] ∧ () = () ∧ True) ∧ ∃ (a0 : Z) (_ : gname), pclos = *[] ∧ tt = tt ∧ () = () ∧ *[a] = *[a0] ∧ (b = a0 ∧ () = ()) ∧ True) P1 True
-      ∧ normalize_conjuncts P1 P2
-      ∧ elim_existentials P2 P3
+    ∃ P1 P2 P3 P4 prog1,
+      bubble_existentials [(∃ pclos : plist id [], True ∧ (∃ (a0 : Z) (_ : gname), pclos = *[] ∧ *[a] = *[a0] ∧ () = () ∧ True) ∧ ∃ (a0 : Z) (_ : gname), pclos = *[] ∧ tt = tt ∧ () = () ∧ *[a] = *[a0] ∧ (b = a0 ∧ () = ()) ∧ True)] [] P1 prog1
+      ∧ normalize_conjuncts P1 P2 true
+      ∧ elim_existentials P2 P3 true
       ∧ unfold_cnf P3 P4
-      ∧ P4 = (b = a).
+      ∧ P4 = (b = a) ∧ prog1 = true.
   Proof.
-    eexists _, _, _, _.
-    split. {  apply _. }
+    eexists _, _, _, _, _.
+    split. { apply _. }
+    simpl.
     split. { apply _. }
     split. { apply _. }
     split; first apply _.
@@ -395,19 +419,27 @@ Section test.
   Abort.
 
   Lemma test2 (a b : Z) :
-    ∃ P,
-      simplify_closure_prop (∃ pclos : plist id [], True ∧ (∃ (a0 : Z) (_ : gname), pclos = *[] ∧ *[a] = *[a0] ∧ () = () ∧ True) ∧ ∃ (a0 : Z) (_ : gname), pclos = *[] ∧ () = () ∧ *[a] = *[a0] ∧ (b = a0 ∧ () = ()) ∧ True) P ∧ P = (b = a).
+    ∃ P prog,
+      simplify_closure_prop (∃ pclos : plist id [], True ∧ (∃ (a0 : Z) (_ : gname), pclos = *[] ∧ *[a] = *[a0] ∧ () = () ∧ True) ∧ ∃ (a0 : Z) (_ : gname), pclos = *[] ∧ () = () ∧ *[a] = *[a0] ∧ (b = a0 ∧ () = ()) ∧ True) P prog ∧ P = (b = a) ∧ prog = true.
   Proof.
-    eexists.
+    eexists _, _.
     split; first apply _.
     done.
   Abort.
 
   Lemma test3 p (b : Z) (clos_states : list (plist (RT_xt ∘ place_rfnRT) [(place_rfn Z * gname)%type : RT])) :
-    ∃ P, simplify_closure_prop (let '(idx, a) := p in ∃ (x : gname) (x0 : Z) (x1 : gname) (x2 : Z), b = a ∧ (x0, x) = (x2, x1) ∧ MinInt i32 ≤ 1 + x0 ∧ 1 + x0 ≤ MaxInt i32 ∧ clos_states !! S idx = Some -[(1 + x2, x1)] ∧ clos_states !! idx = Some -[(x0, x)]) P ∧ P = P.
+    ∃ P, simplify_closure_prop (let '(idx, a) := p in ∃ (x : gname) (x0 : Z) (x1 : gname) (x2 : Z), b = a ∧ (x0, x) = (x2, x1) ∧ MinInt i32 ≤ 1 + x0 ∧ 1 + x0 ≤ MaxInt i32 ∧ clos_states !! S idx = Some -[(1 + x2, x1)] ∧ clos_states !! idx = Some -[(x0, x)]) P true ∧ P = P.
   Proof.
     eexists. split; first apply _.
     simpl.
+  Abort.
+
+  Lemma test4 (a b : Z) :
+    ∃ P prog, simplify_closure_prop (a = b) P prog ∧ prog = false ∧ P = P.
+  Proof.
+    eexists _, _. split; first apply _.
+    simpl.
+    done.
   Abort.
 End test.
 
@@ -509,8 +541,8 @@ End simplify_relation.
 Existing Class simplify_relation.
 Existing Class simplify_relation_functional.
 
-Existing Instance simplify_relation_prod | 100.
-Existing Instance simplify_relation_atom | 10.
+Existing Instance simplify_relation_prod | 10.
+Existing Instance simplify_relation_atom | 100.
 Existing Instance simplify_relation_atom_keep | 1000.
 Existing Instance simplify_relation_functional_eq | 10.
 Existing Instance simplify_relation_functional_function | 11.
@@ -518,12 +550,12 @@ Existing Instances simplify_relation_prod_unit_l simplify_relation_prod_unit_r |
 
 Definition simplify_relation_passes := simplify_relation.
 
-Lemma simplify_relation_make_pass A B C1 C2 Φ Φ' Ψ1 Ψ2 map_C1 map_C2 Ψ3 prog1 prog2 :
-  (∀ a b, simplify_closure_prop (Φ a b) (Φ' a b)) →
+Lemma simplify_relation_make_pass A B C1 C2 Φ Φ' Ψ1 Ψ2 map_C1 map_C2 Ψ3 prog0 prog1 prog2 prog3 :
+  (∀ a b, simplify_closure_prop (Φ a b) (Φ' a b) prog0) →
   simplify_relation A B Φ' C1 Ψ1 map_C1 prog1 →
   simplify_relation A C1 Ψ1 C2 Ψ2 map_C2 prog2 →
-  (∀ a c2, simplify_closure_prop (Ψ2 a c2) (Ψ3 a c2)) →
-  simplify_relation_passes A B Φ C2 Ψ3 (λ a c2, map_C1 a (map_C2 a c2)) (prog1 || prog2).
+  (∀ a c2, simplify_closure_prop (Ψ2 a c2) (Ψ3 a c2) prog3) →
+  simplify_relation_passes A B Φ C2 Ψ3 (λ a c2, map_C1 a (map_C2 a c2)) (prog0 || prog1 || prog2 || prog3).
 Proof.
   unfold simplify_relation_passes, simplify_relation.
   naive_solver.
@@ -572,6 +604,16 @@ Section test.
     { apply _.  }
     simpl.
   Abort.
+
+  Lemma test4 :
+    ∃ C Ψ map_C prog, simplify_relation_passes _ _ (λ (a : Z * gname) (b : Z), ∃ pclos : plist id [], True ∧ (∃ (a0 : Z * gname) (_ : gname), pclos = *[] ∧ *[a] = *[a0] ∧ () = () ∧ a0.1 = 5 ∧ True) ∧ ∃ (a0 : Z * gname) (_ : gname), pclos = *[] ∧ () = () ∧ *[a] = *[a0] ∧ (∃ a1 : Z, b = a1 ∧ a1 = a0.1 ∧  True ∧ () = ()) ∧ True)
+      C Ψ map_C prog ∧ Ψ = Ψ.
+  Proof.
+    eexists _, _, _ ,_.
+    split. { apply _. }
+    simpl.
+  Abort.
+
 End test.
 
 Lemma Forall2_simplify_relation {A B} (Φ : A → B → Prop) l1 l2 C Ψ map_C prog :
@@ -598,13 +640,19 @@ Proof.
     eauto.
 Qed.
 
-Global Instance simpl_impl_Forall2_simplify A B C Φ Ψ map_C l1 l2 :
-  simplify_relation A B Φ C Ψ map_C true →
-  SimplImpl true (Forall2 Φ l1 l2) (λ T, (∃ l3, l2 = fmap (λ '(a, c), map_C a c) (zip l1 l3) ∧ Forall2 Ψ l1 l3) → T).
+(* TODO: maybe we can simplify a bit more here. *)
+Lemma simpl_impl_Forall2_simplify A B C Φ Ψ map_C l1 l2 prog :
+  simplify_relation_passes A B Φ C Ψ map_C prog →
+  prog = true →
+  SimplImpl prog (Forall2 Φ l1 l2) (λ T, (∃ l3, l2 = fmap (λ '(a, c), map_C a c) (zip l1 l3) ∧ Forall2 Ψ l1 l3) → T).
 Proof.
-  intros Hsimpl T.
-  rewrite Forall2_simplify_relation; done.
+  intros Hsimpl _ T.
+  unfold simplify_relation_passes in Hsimpl.
+  rewrite Forall2_simplify_relation. done.
 Qed.
+Global Hint Extern 10 (SimplImpl _ (Forall2 _ _ _) _) =>
+  notypeclasses refine (simpl_impl_Forall2_simplify _ _ _ _ _ _ _ _ _ _ _);
+  [typeclasses eauto | done ] : typeclass_instances.
 
 Global Instance simpl_impl_Forall2_unit_r {A} (Φ : A → Prop) l1 (l2 : list unit) :
   SimplImpl true (Forall2 (λ a _, Φ a) l1 l2) (λ T, l2 = replicate (length l1) tt → Forall Φ l1 → T).
